{\allowdisplaybreaks
\begin{align*}
\cfrac{1}{1 - x}  &=  1 + x + x^2 + x^3 + x^4 + \cdots    &=  \sum_{i=0}^\infty x^i \\
\cfrac{1}{1 - c x}  &=  1 + c x + c^2 x^2 + c^3 x^3 + \cdots  &=  \sum_{i=0}^\infty c^i x^i \\
\cfrac{1}{1 - x^n}  &=  1 + x^n + x^{2n} + x^{3n} + \cdots    &=  \sum_{i=0}^\infty x^{ni} \\
\cfrac{x}{(1 - x)^2}&=  x + 2 x^2 + 3 x^3 + 4 x^4 + \cdots    &=  \sum_{i=0}^\infty i x^i \\
\sum_{k=0}^n \stls{n}{k} \cfrac{k! z^k}{(1-z)^{k+1}}
          &=  x + 2^n x^2 + 3^n x^3 + 4^n x^4 + \cdots
                                &=  \sum_{i=0}^\infty i^n x^i \\
e^x          &= 1 + x + \cfrac{1}{2} x^2 + \cfrac{1}{6} x^3 + \cdots
                                &=  \sum_{i=0}^\infty \cfrac{x^i}{i!} \\
\ln (1 + x)      &=  x - \cfrac{1}{2} x^2 + \cfrac{1}{3} x^3 - \cfrac{1}{4} x^4  - \cdots
                                &=  \sum_{i=1}^\infty (-1)^{i+1} \cfrac{x^i}{i} \\
\ln \cfrac{1}{1 - x}
          &=  x + \cfrac{1}{2} x^2 + \cfrac{1}{3} x^3 + \cfrac{1}{4} x^4  + \cdots
                                &=  \sum_{i=1}^\infty \cfrac{x^i}{i} \\
\sin x        &=  x - \cfrac{1}{3!} x^3  + \cfrac{1}{5!} x^5 - \cfrac{1}{7!} x^7 +  \cdots
                                &=  \sum_{i=0}^\infty (-1)^i \cfrac{x^{2i+1}}{(2i+1)!} \\
\cos x        &=  1 - \cfrac{1}{2!} x^2  + \cfrac{1}{4!} x^4 - \cfrac{1}{6!} x^6 +  \cdots
                                &=  \sum_{i=0}^\infty (-1)^i \cfrac{x^{2i}}{(2i)!} \\
\tan^{-1} x      &=  x - \cfrac{1}{3} x^3  + \cfrac{1}{5} x^5 - \cfrac{1}{7} x^7 +  \cdots
                                &=  \sum_{i=0}^\infty (-1)^i \cfrac{x^{2i+1}}{(2i+1)} \\
(1+x)^n        &=  1 + n x + \cfrac{n(n-1)}{2} x^2 +  \cdots
                                &=  \sum_{i=0}^\infty {n \choose i} x^i \\
\cfrac{1}{(1-x)^{n+1}}
          &=  1 + (n+1) x + {n+2 \choose 2} x^2 +  \cdots
                                &=  \sum_{i=0}^\infty {i+ n \choose i} x^i \\
\cfrac{x}{e^x - 1}  &=  1 - \cfrac{1}{2} x + \cfrac{1}{12} x^2 - \cfrac{1}{720} x^4 + \cdots
                                &=  \sum_{i=0}^\infty \cfrac{B_i x^i}{i!} \\
\cfrac{1}{2x}(1 - \sqrt{1-4x})
          &=  1 + x + 2 x^2 + 5 x^3 +  \cdots
                                &=  \sum_{i=0}^\infty \cfrac{1}{i+1}{2i \choose i}x^i \\
\cfrac{1}{\sqrt{1-4x}}
          &=  1 + 2 x + 6 x^2 + 20 x^3 + \cdots
                                &=  \sum_{i=0}^\infty {2i \choose i}x^i \\
\cfrac{1}{\sqrt{1-4x}}\left(\cfrac{1 - \sqrt{1-4x}}{2x}\right)^n
          &=  1 + (2+n)x + {4+n \choose 2} x^2 + \cdots
                                &=  \sum_{i=0}^\infty {2i+n \choose i}x^i \\
\cfrac{1}{1-x}\ln\cfrac{1}{1 - x}
          &=  x + \cfrac{3}{2} x^2 + \cfrac{11}{6} x^3 + \cfrac{25}{12} x^4 + \cdots
                                &=  \sum_{i=1}^\infty H_i x^i \\
\cfrac{1}{2}\left(\ln\cfrac{1}{1- x}\right)^2
          &=  \cfrac{1}{2} x^2 + \cfrac{3}{4} x^3 + \cfrac{11}{24} x^4 + \cdots
                                &=  \sum_{i=2}^\infty \cfrac{H_{i-1} x^i}{i} \\
\cfrac{x}{1 - x - x^2}
          &=  x + x^2 + 2 x^3 + 3 x^4 +  \cdots
                                &=  \sum_{i=0}^\infty F_i x^i \\
\cfrac{F_n x}{1 - (F_{n-1} + F_{n+1})x - (-1)^n x^2}
          &=  F_n x + F_{2n} x^2 + F_{3n} x^3 + \cdots
                                &=  \sum_{i=0}^\infty F_{ni} x^i
\end{align*}
}
